\documentclass{article}
\usepackage[utf8]{inputenc}
\usepackage[papersize={8.5in,11in},margin=0.8in]{geometry}
\usepackage{amsfonts}
\usepackage{amsmath}
\usepackage{amssymb}
\usepackage{xcolor}
\usepackage{color, colortbl}

\title{Math 505 Assignment 6}
\author{John Caruthers}
\date\today

\begin{document}
\maketitle

Prove by induction.
\begin{itemize}

    \item[1.] \textbf{Theorem 15:} If $n$ is a natural number, then $1+2+3+...+n=\frac{n(n+1)}{2}$
    
    \begin{itemize}
        \item[]\emph{Basis:} $n=1$ so, $1=\frac{1(1+1)}{2}=\frac{2}{2}=1$.
        
        \item[]\emph{Inductive Hypothesis:} $n=k$, so $1+2+3+...+k=\frac{k(k+1)}{2}$.
        
        \item[]\emph{Inductive Step:} $n=k+1$, so $1+2+3+...+k+(k+1)=\frac{(k+1)(k+2)}{2}$.
        
        \begin{align}
            \frac{k(k+1)}{2}+(k+1)&=\frac{(k+1)(k+2)}{2}\nonumber\\
            \frac{k(k+1)+2(k+1)}{2}&=\frac{(k+1)(k+2)}{2}\nonumber\\
            \frac{(k+1)(k+1)}{2}&=\frac{(k+1)(k+2)}{2}\nonumber
        \end{align}
        By induction, If $n$ is a natural number, then $1+2+3+...+n=\frac{n(n+1)}{2}$. $\Box$
        
        {\color{blue} Upon review, this proof is exactly like what was performed in Chapter 3, no corrections needed.}
        
    \end{itemize}
    
    \item[2.] \textbf{Theorem 16:} For all positive integers $n$, $1+2^1+2^2+...+2^n=2^{n+1}-1$.
    
    \begin{itemize}
        \item[]\emph{Basis:} $n=1$, so $1+2^1=2^{1+1}-1=3$.
        
        \item[]\emph{Inductive Hypothesis:} $n=k$, so $1+2^1+2^2+...+2^k=2^{k+1}-1$.
        
        \item[]\emph{Inductive Step:} $n=k+1$, so $1+2^1+2^2+...+2^k+2^{k+1}=2^{k+2}-1$.
        
        \begin{align}
            2^{k+1}-1&=2^{k+2}-1\nonumber\\
            2(2^{k+1})-1&=2^{k+2}-1\nonumber\\
            2^{k+2}-1&=2^{k+2}-1\nonumber
        \end{align}
        By induction, For all positive integers $n$, $1+2^1+2^2+...+2^n=2^{n+1}-1$.
        
        {\color{blue} Upon review, this proof is exactly like what was performed in Chapter 3, no corrections needed.}
    \end{itemize}
    
\end{itemize}

\end{document}
